Proved well-formed for cbn, important for bisimulation relation

cbn.v
@@ -1,18 +1,10 @@
 (* Based on figure 8 of ariola et al *) 
-Require Import Lists.List.
+Require Import Lists.List Decidable CpdtTactics Program.Basics.
 Require Import Unicode.Utf8_core.
 Require Import expr util.
 Require Import Arith.Peano_dec.
 
 Definition heap := list (nat * tm). 
-
-Fixpoint InDomain (i:nat) (h:heap) : Prop := match h with
-  | cons (j,_) tail => j = i \/ InDomain i tail
-  | nil => False
-  end.
-
-Example k : InDomain 3 (cons (4,var 3) (cons (3, var 4) nil)).
-Proof. simpl. right. left. reflexivity. Qed. 
 
 Inductive configuration : Type := 
   | st : heap -> tm -> configuration.
@@ -23,14 +15,9 @@ Notation " ⟨ Ψ , b ⟩ N " := (st (cons b Ψ) N) (at level 40).
 Notation " ⟨ Φ , b , Ψ ⟩ N " := (st (Datatypes.app Ψ (cons b Φ)) N) (at level 40).
 
 Definition domain (h:heap) : list nat := @map (nat * tm) nat (@fst nat tm) h.
-
-Lemma head_elem : forall h tail,  elem h (cons h tail).
-  intros. simpl. left. reflexivity. Qed.
-
-Definition fresh (n : nat) (e : tm) (h : heap) (d : list nat) := 
-  ~ elem n d
-  /\ ~ elem n (fvs e)
-  /\ ~ elem n (domain h).
+Definition fresh (n : nat) (e : tm) (h : heap) (d : list nat) := ~ In n d
+  /\ ~ In n (vars e)
+  /\ ~ In n (domain h).
 
 (* Direct description of Maraist et al. Figure 8, with amendment from  *)
 Reserved Notation " c1 '⇓' d '#' c2 " (at level 50).
@@ -47,6 +34,138 @@ where " c1 '⇓' d '#' c2 " := (step c1 d c2).
 
 Lemma values_only : ∀ c M Ψ d, c ⇓ d # ⟨Ψ⟩M -> value M.
 intros. inversion H; simpl; auto. Qed. 
+
+Definition closed_under (c : configuration) : Prop := match c with
+  | st h t => subset (fvs t) (domain h) end.
+
+Definition closed (t : tm) : Prop := closed_under (st nil t).
+
+Fixpoint well_formed_heap (h : heap) : Prop := match h with
+  | cons (x, M) t => closed_under (st t M)  /\ well_formed_heap t 
+  | nil => True
+  end.
+
+Definition well_formed (c : configuration) : Prop := match c with 
+  | st h t => closed_under c /\ well_formed_heap h 
+  end.
+
+Fixpoint collapse (h : heap) : tm -> tm :=  match h with
+  | nil => id 
+  | cons (x, e') t => compose (subst x (collapse t e')) (collapse t)
+  end.
+
+Example collapse_simple : collapse (0↦:λ0, 0  :: nil) 0 = :λ0, 0.
+eauto. Qed. 
+
+Lemma well_formed_app : ∀ (Φ Ψ:heap) (x:nat) (M N:tm), 
+  well_formed (⟨Φ, x ↦ M, Ψ⟩N) ->
+  well_formed (⟨Φ⟩ M).
+intros. 
+destruct H.  
+clear H.
+induction Ψ.
+destruct H0. split; assumption. simpl in H0. apply IHΨ.
+destruct a. destruct H0. assumption.  Qed.
+
+Definition stheap (c:configuration) : heap := match c with | st h t => h end.
+Definition sttm (c:configuration) : tm := match c with | st h t => t end.
+
+Lemma well_formed_collapse : forall h, well_formed_heap h -> 
+  ∀ n t, In n (fvs (collapse h t)) -> In n (fvs t) /\ ~In n (domain h).
+intros h wf. induction h. crush. destruct a. intros. simpl in wf. destruct wf.
+simpl in H. unfold compose in H.  assert (subset (fvs ([collapse h t //
+n]collapse h t0)) (fvs (collapse h t) ++ remove n (fvs (collapse h t0)))). apply
+subst_subset. rewrite <- subset_eq in H2. apply H2 in H. clear H2. rewrite in_app_iff in
+H. destruct H.  rewrite <- subset_eq in H0. apply IHh in H. crush. assumption. 
+destruct (eq_nat_dec n0 n). subst. apply remove_in in H. inversion H. apply
+remove_not_in in H. apply IHh in H. crush. assumption. assumption. Qed.
+
+Lemma well_formed_collapse_closed : forall h t, well_formed_heap h ->
+closed_under (st h t) -> closed (collapse h t).
+intros. assert (∀ n t, In n (fvs (collapse h t)) -> In n (fvs t) /\ ~In n
+(domain h)). apply well_formed_collapse. assumption. unfold closed. unfold
+closed_under. simpl. rewrite <- subset_eq. unfold subset'. intros. apply H1 in
+H2. simpl. destruct H2. unfold closed_under in H0. rewrite <- subset_eq in H0.
+apply H0 in H2. apply H3 in H2. assumption. Qed. 
+
+Lemma not_vars_fvs : forall n e, ~(In n (vars e)) -> ~(In n (fvs e)).
+induction e. simpl. intros. assumption. simpl. rewrite in_app_iff. rewrite
+in_app_iff. intros. apply not_or in H. destruct H. apply IHe1 in H. apply IHe2
+in H0. unfold not. intros. destruct H1. apply H in H1. assumption. apply H0 in
+H1. assumption. simpl. intros. apply not_or in H. destruct H. apply IHe in H0.
+unfold not. intros. unfold not in H. assert (n <> n0). unfold not. intros.
+symmetry in H2.  apply H in H2. assumption. apply remove_not_in with (ns:=fvs e)
+in H2. apply H2 in H1. apply H0 in H1. assumption. Qed.  
+
+Lemma fresh_subst : forall x x' e h d, fresh x' e h d -> fvs ([x'//x]e) = replace x x' (fvs e).
+intros. destruct H. destruct H0. induction e. simpl in H0. apply not_or in H0.
+destruct H0. simpl. unfold replace'. destruct (eq_nat_dec x n); simpl; auto. simpl. unfold
+replace. rewrite map_app. simpl in H0. rewrite in_app_iff in H0. apply
+not_or in H0. destruct H0. apply IHe1 in H0. apply IHe2 in H2. rewrite H0.
+rewrite H2. reflexivity. simpl. destruct (eq_nat_dec x n). simpl. subst. rewrite
+replace_remove. auto.  simpl. simpl in H0. apply not_or in H0. destruct H0.
+assert (not (In x' (fvs e))). apply not_vars_fvs in H2. assumption.
+apply IHe in H2. rewrite H2. induction (fvs e). auto. simpl. simpl in H2. unfold
+replace' in H2. unfold replace'. 
+destruct (eq_nat_dec x a). destruct (eq_nat_dec n x'). apply H0 in e1. inversion
+e1. destruct (eq_nat_dec n a). subst. rewrite replace_remove. assert (a = a).
+reflexivity. apply n0 in H4. inversion H4. subst. simpl. unfold replace'. rewrite
+eq_nat_dec_refl. simpl in H3. apply not_or in H3. destruct H3. apply
+remove_replace_comp with (y:=a) (z:=n) in H4 . rewrite H4. reflexivity.
+assumption. assumption. unfold not. intros. simpl in H3. apply not_or in H3. destruct H3. destruct (eq_nat_dec n
+a). subst. apply remove_replace_comp. assumption. assumption. unfold not.
+intros. symmetry in H5. apply n0 in H5. assumption. simpl. unfold replace'. destruct (eq_nat_dec
+x a). apply n1 in e0. inversion e0. apply remove_replace_comp with (y:=x)
+(z:=n) in H4. rewrite H4. reflexivity. assumption. auto. Qed. 
+
+Lemma monotonic_heap : forall c1 c2 d, c1 ⇓ d # c2 -> 
+subset (domain (stheap c1)) (domain (stheap c2)).  
+intros. 
+induction H. 
+simpl.  simpl in IHstep. unfold domain. rewrite map_app. rewrite map_app. unfold
+domain in IHstep. simpl. apply subset_comm1. simpl. split. apply
+in_or_app. right. simpl. auto. 
+apply subset_comm1. simpl. apply subset_app_id. apply subset_cons. assumption.
+apply subset_id. simpl. simpl in IHstep1. simpl in IHstep2. destruct IHstep2.
+apply subset_trans with (ys:=domain Ψ); assumption. Qed.
+
+Lemma well_formed_var : forall Φ Ψ Υ x n v, well_formed (⟨Ψ, x↦n, Υ⟩x) -> subset
+  (domain Ψ) (domain Φ) -> well_formed (⟨Φ⟩v) -> well_formed (⟨Φ, x↦v, Υ⟩v).
+intros. split. simpl. unfold domain. rewrite map_app. apply subset_comm2. apply
+subset_app.  apply subset_cons. destruct H1. unfold closed_under in H1.
+assumption. inversion H as [H' H2].  induction Υ. simpl. destruct H1. unfold
+closed_under in H1. split; assumption.  destruct a. simpl in H2. destruct H2.
+simpl. split. unfold domain. rewrite map_app.  unfold domain in H2. rewrite
+map_app in H2.  apply subset_comm2 in H2. simpl in H2. apply subset_comm2.
+simpl.  rewrite cons_app. rewrite cons_app in H2. rewrite app_comm_cons.
+rewrite app_comm_cons in H2. apply subset_comm2. rewrite <- app_assoc. apply
+subset_comm2 in H2.  rewrite <- app_assoc in H2. apply subset_comm2. apply
+subset_comm2 in H2.  unfold domain in H0. apply subset_app_id with (xs :=
+((((map (fst (B:=tm)) Υ ++ x :: nil))))) in H0. apply subset_trans with (ys :=
+((map (fst (B:=tm)) Υ ++ x :: nil) ++ map (fst (B:=tm)) Ψ)). assumption.
+assumption.  apply well_formed_app in H.  destruct H. clear H'. clear H4. unfold
+closed_under in H. apply subset_app with (zs:=domain (Υ ++ x↦n :: nil)) in H.
+assert (well_formed (⟨Ψ, x ↦n, Υ ⟩ x)). split. unfold closed_under. unfold
+domain.  rewrite map_app. apply subset_comm2. simpl. auto. assumption. apply
+IHΥ.  assumption. destruct H4. assumption. assumption. Qed.
+
+Theorem well_formed_step : ∀ c1 c2 d, well_formed c1 -> c1 ⇓ d # c2 -> well_formed c2.
+intros. induction H0. assert (well_formed (⟨Φ, x ↦ M, Υ⟩x)). assumption. split. 
+apply well_formed_app in H. apply IHstep in H. unfold closed_under. 
+unfold domain. rewrite map_app. apply subset_comm2. apply
+subset_app. apply subset_cons.  destruct H. assumption. 
+apply monotonic_heap in H0. simpl in H0. apply well_formed_var with (Ψ:=Φ)
+(Φ:=Ψ) (x:=x) (v:=:λy,N) in H. inversion H. assumption. assumption. apply
+well_formed_app in H. apply IHstep in H. assumption. assumption. 
+destruct H. unfold closed_under in H. simpl in H. apply app_subset_and in H. destruct H.
+assert (well_formed (⟨Φ ⟩ L)). split; assumption. assert (well_formed (⟨Φ ⟩ M)).
+split; assumption. apply IHstep1 in H3.  assert (well_formed (⟨Ψ, x' ↦ M ⟩ [x'
+// x]N)). split. unfold closed_under. simpl. apply fresh_subst with (x:=x) in
+H0. rewrite H0. apply replace_cons. destruct H3. simpl in H3. apply subset_remove_cons
+in H3. assumption.  apply monotonic_heap in H0_. simpl in H0_. split. unfold
+closed_under. destruct H4. unfold closed_under in H4. apply subset_trans with
+(ys:=domain Φ); assumption. destruct H3. assumption. apply IHstep2 in H5.
+assumption. Qed.
 
 Example simple : (step (⟨nil⟩ ((:λ0,0) @ (:λ0,0))) nil (⟨nil, 1 ↦ :λ0,0⟩ :λ0,0)).
 apply App with 0 0 1 nil nil. unfold fresh.  simpl. split; auto. split. unfold
