db.v
@@ -1,66 +1,77 @@
+Require Import Decidable.
 Require expr expr_db_nat.
 Require Import List Datatypes util.
+Require Import FunctionalExtensionality CpdtTactics. 
+Require Import Arith.Peano_dec.
+Require Import Program.Basics.
 Set Implicit Arguments.
 
-Definition fmap_succ (p : prod nat nat) : prod nat nat := match p with
-  | (a,b) => (a, S b)
-  end.
-  
-(* a relation between standard lambda terms and deBruijn-indexed terms*)
+(* db.v : used to relate debruijn terms with standard terms *) 
+
+
+Definition fmap {A B C} (f : B -> C) : A * B -> A * C  := fun x => match x with
+  | (a, b) => (a, f b) end. 
+
+(* a relation between standard lambda terms and deBruijn-indexed term, note that
+  standard variables are nats as well *)
 Inductive db : expr.tm -> list (prod nat nat) -> expr_db_nat.expr -> Prop :=
   | dbVar : forall bs cs v i, 
       db (expr.var v) (bs ++ (v, i) :: cs) (expr_db_nat.var i)
   | dbAbs : forall bs v b b',
-      db b ((v,0) :: map fmap_succ bs) b' ->
+      db b ((v,0) :: map (fmap S) bs) b' ->
       db (expr.abs v b) bs (expr_db_nat.lam b')
   | dbApp : forall m n m' n' bs,
       db m bs m' ->
       db n bs n' ->
       db (expr.app m n) bs (expr_db_nat.app m' n').
 
+(* debruijn relation for closed terms *)
 Definition deBruijn (t:expr.tm) (e:expr_db_nat.expr) : Prop := db t nil e.
-
-Lemma elem_app : forall x xs ys, elem x (List.app xs ys) <-> 
-                                 (elem x xs \/ elem x ys).
-intros. induction xs. simpl. split; intros. apply or_intror. assumption.
-apply or_false in H. assumption. simpl. rewrite IHxs. split;  intros. rewrite
-or_assoc. assumption. rewrite or_assoc in H. assumption. Qed.
 
 Lemma let_inline :forall (b c:prod nat nat),
     (fst (let a := b in c)) = (let a := b in fst c).
     auto. Qed.
 
-Lemma fst_fmap_succ : forall x, fst (fmap_succ x) = fst x.
-intros. destruct x. simpl. reflexivity. Qed. 
-
-Lemma fst_map_fmap_succ : forall xs:list (prod nat nat), map (fun x => fst
-(fmap_succ x)) xs = map (@fst nat nat) xs.
-intros. induction xs. auto. simpl. rewrite IHxs. auto. rewrite fst_fmap_succ.
-auto. Qed.  
-
 Definition domain (A B : Type) : list (prod A B) -> list A := map (@fst A B). 
 
-Theorem db_closed_tm : forall f t e, db t f e -> subset (expr.fvs t) (domain f).
-  intros. 
-  induction H.
-  simpl.
-  unfold domain.
-  rewrite map_app. 
-  simpl. 
-  rewrite elem_app. 
-  simpl. 
-  split. 
-  right. left. 
-  reflexivity. 
-  apply I. 
-  simpl. simpl in IHdb. 
-  unfold domain in IHdb.
-  rewrite map_map in IHdb. 
-  rewrite fst_map_fmap_succ in IHdb.  
-  apply subset_filter_cons. assumption.
-  simpl.  
-  apply app_subset. split; assumption. 
+
+Lemma domain_fmap : forall A B C (f:B->C) (xs:list (A * B)),  domain (map
+(fmap f) xs) = domain xs.
+intros. induction xs. crush. crush. Qed. 
+
+Theorem db_closed_under : forall f t e, db t f e -> subset (expr.fvs t) (domain f).
+intros.  induction H.  simpl.  unfold domain.  rewrite map_app.  simpl.
+split.  apply in_or_app.  simpl.  right. left.  reflexivity.  apply I.  simpl.
+simpl in IHdb.  rewrite domain_fmap in IHdb. rewrite <-
+subset_remove_cons. assumption. simpl. apply app_subset_and. split; assumption.
 Qed. 
+
+Theorem db_closed : forall t e, db t nil e -> expr.fvs t = nil.
+intros. apply db_closed_under in H. simpl in H. unfold subset in H. destruct
+(expr.fvs t).  reflexivity. inversion H. inversion H0. Qed. 
+
+(*
+Theorem closed_db_under : forall f t e, subset (expr.fvs t) (domain f) -> db t f e.
+intros. induction f. crush. induction db. 
+induction e. crush. apply in_split in H0. destruct H0. destruct H.   
+induction H. crush. unfold domain. rewrite map_app. rewrite in_app_iff.
+right. crush. crush. rewrite <- subset_remove_cons. rewrite domain_fmap in IHdb.
+assumption. simpl. apply app_subset_and. crush. Qed. 
+*)
+
+
+Definition lookup' {A B} : forall (f : list (A * B)) (a: {a | In a (domain f)}), B. 
+intros. induction f. crush. destruct a. inversion f. destruct a0. assumption.
+Qed.
+
+Definition In' {A} := flip (@In A).
+
+Definition sumbool_or {A B} : {A} + {B} -> A \/ B := fun b => match b with
+  | left a => or_introl a
+  | right b => or_intror b
+  end.
+
+Definition inx (x:nat) := In x (domain ((0,1) :: nil)).
 
 Lemma in_heap : forall (A B : Type) (k : A) (f : list (prod A B)), In k (domain f)
                          -> (exists v, In (k,v) f).
@@ -68,8 +79,7 @@ intros. unfold domain in H. apply in_map_iff with (prod A B) A (@fst A B) f k in
 H. destruct H.  destruct H. destruct H. destruct x. simpl. apply ex_intro with
 b. assumption. Qed. 
 
-(* id = id *)
-Lemma ex1 : db (expr.abs 0 (expr.var 0)) nil (expr_db_nat.lam (expr_db_nat.var 0)).
+(* id = id *) Lemma ex1 : db (expr.abs 0 (expr.var 0)) nil (expr_db_nat.lam (expr_db_nat.var 0)).
 apply dbAbs. simpl. rewrite <- app_nil_l with (prod nat nat) ((0, 0) :: nil).
 apply dbVar. Qed.
 
