expr.v
@@ -1,5 +1,6 @@
-Require Import FSets.FSetInterface List util.
+Require Import FSets.FSetInterface util EqNat Sumbool Decidable.
 Require Import Arith.Peano_dec.
+Require Import CpdtTactics.
 
 Inductive tm : Type :=
   | var : nat -> tm
@@ -16,18 +17,90 @@ Notation " M @ N " := (app M N) (at level 60).
 Coercion var : nat >-> tm.
 
 Fixpoint fvs (e:tm) : list nat := match e with
-  | var v => cons v nil
-  | abs v b => filter (compose negb (neq_bool v)) (fvs b)
-  | app m n => List.app (fvs m) (fvs n)
+  | var v =>  v::nil
+  | abs v b => remove v (fvs b)
+  | app m n => fvs m ++ fvs n
+  end.
+
+Fixpoint vars (e:tm) : list nat := match e with
+  | var v => v::nil
+  | abs v b => v::vars b
+  | app m n => vars m ++ vars n
   end.
 
 Reserved Notation "'[' x '//' y ']' t" (at level 20).
 Fixpoint subst (x : nat) (x' : tm) (t : tm) : tm := match t with
-  | var y => if eq_nat_dec y x then x' else t
+  | var y => if eq_nat_dec x y then x' else t
   | m@n => [x'//x]m @ [x'//x]n
-  | :λy,b => if eq_nat_dec y x then t else (:λy,[x'//x]b)
+  | :λy,b => if eq_nat_dec x y then t else :λy,([x'//x]b) 
   end
 where " '[' x '//' y ']' t " := (subst y x t).
+
+Lemma subst_subset : forall t m x, subset (fvs ([t//x]m)) (fvs t ++ remove x (fvs m)).
+intros. induction m. simpl. destruct (eq_nat_dec x n); crush. apply subset_app.
+apply subset_id. simpl. rewrite app_subset_and. split. rewrite remove_app. rewrite app_assoc. apply
+subset_app. assumption. apply subset_comm2. rewrite remove_app. rewrite <- app_assoc. apply
+subset_comm2. apply subset_app. apply subset_comm2. assumption. simpl. destruct
+(eq_nat_dec x n). simpl. subst. apply subset_comm2. apply subset_app. rewrite
+remove_idem. apply
+subset_id. simpl. rewrite <- subset_remove_cons. rewrite <- subset_eq in IHm.
+rewrite <- subset_eq.  unfold subset'. intros. unfold subset' in IHm. apply IHm
+in H. simpl.  rewrite in_app_iff in H. destruct H. right. rewrite in_app_iff.
+left. assumption. destruct (eq_nat_dec n a). left. assumption. right. rewrite
+in_app_iff. right. rewrite remove_dup. apply remove_not_in with (ns:=remove x (fvs m)). auto. assumption. Qed. 
+
+Lemma fvs_lam_dom : forall v b d, subset (fvs (abs v b)) d <-> subset (fvs b) (v :: d). 
+intros. split; intros. simpl in H. rewrite subset_remove_cons. assumption.
+simpl. rewrite <- subset_remove_cons. assumption. Qed.
+
+Definition replace' : nat -> nat -> nat -> nat := fun y z x => if eq_nat_dec y x then z else x.
+Definition replace (y z:nat) := map (replace' y z).
+
+Lemma replace_not_in : forall x x' xs, x <> x' -> ~In x (replace x x' xs).
+intros. unfold not. induction xs. auto. simpl. unfold replace'. destruct (eq_nat_dec x a). 
+intros. destruct H0. symmetry in H0. auto. auto. intros. 
+destruct H0. symmetry in H0. auto. auto. Qed. 
+
+Lemma replace_remove : forall x x' xs, replace x x' (remove x xs) = remove x xs.
+intros. induction xs. auto. simpl. destruct (eq_nat_dec x a). assumption. simpl.
+unfold replace'. 
+destruct (eq_nat_dec x a). apply n in e. inversion e. rewrite IHxs. reflexivity.
+Qed. 
+
+Lemma remove_replace_comp : forall x y z zs, ~In x zs -> z <> x -> z <> y ->  
+(remove z (replace y x zs) = replace y x (remove z zs)). intros. induction zs.
+auto. simpl in H.  apply not_or in H. destruct H. simpl. destruct (eq_nat_dec y
+a). unfold replace'. subst. rewrite eq_nat_dec_refl. destruct (eq_nat_dec z x).
+apply H0 in e. inversion e. destruct (eq_nat_dec z a). apply H1 in e. inversion
+e. simpl. unfold replace'. apply IHzs in H2. rewrite eq_nat_dec_refl. rewrite
+H2. reflexivity.  unfold replace'. simpl. destruct (eq_nat_dec z a). subst.
+apply IHzs in H2. rewrite H2. destruct (eq_nat_dec y a). apply n in e. inversion
+e. rewrite eq_nat_dec_refl. reflexivity. simpl.  unfold replace'. destruct
+(eq_nat_dec y). destruct (eq_nat_dec z x). apply H0 in e0. inversion e0. apply
+IHzs in H2. rewrite H2. reflexivity. simpl. destruct (eq_nat_dec z a). apply n0
+in e. inversion e. apply IHzs in H2. rewrite H2. reflexivity.  Qed. 
+
+Lemma replace_imp : forall x y xs, In x xs -> In y (replace x y xs). 
+intros. unfold replace. assert (y = replace' x y x). unfold replace'. rewrite
+eq_nat_dec_refl. reflexivity. rewrite H0 at 1.  apply in_map. assumption. 
+Qed.
+  
+Lemma replace_id : forall x xs, replace x x xs = xs. 
+intros. induction xs. auto. simpl. unfold replace'. destruct (eq_nat_dec x a). rewrite <- e. rewrite
+IHxs. reflexivity. rewrite IHxs. reflexivity. Qed. 
+
+Lemma replace_in : forall x y a xs, a <> y -> In a (replace x y xs) -> In a xs.
+intros. destruct (eq_nat_dec a x). subst. apply replace_not_in with
+(xs:=xs) in H. apply H in H0. inversion H0. induction xs. auto. simpl in H0.
+simpl. destruct H0. unfold replace' in H0. destruct (eq_nat_dec x a0); simpl;
+crush. crush. Qed.  
+
+Lemma replace_cons : forall x x' xs ys, subset xs (x::ys) -> subset (replace x x' xs) (x'::ys). 
+intros. destruct (eq_nat_dec x x'). subst. rewrite replace_id. assumption.
+induction xs. simpl. auto. simpl in H. destruct H. destruct H. subst. apply IHxs
+in H0. simpl. split. unfold replace'. rewrite eq_nat_dec_refl. left.
+reflexivity. assumption. apply IHxs in H0. simpl. split. unfold replace'. destruct (eq_nat_dec x
+a). left; reflexivity. right. assumption. assumption. Qed. 
 
 Lemma ex1 : fvs (var 1) = cons 1 nil.
 simpl. reflexivity. Qed.
