util.v
@@ -1,65 +1,160 @@
-Require Import List Basics.
-
-Fixpoint elem (n: nat) (d: list nat) : Prop := match d with
-  | nil => False
-  | cons m ms => n = m \/ elem n ms
-  end.
-
-Fixpoint neq_bool (n m : nat) : bool := match n,m with
-  | 0,0 => true
-  | 0,S m' => false
-  | S _, 0 => false
-  | S n', S m' => neq_bool n' m'
-  end.
-
-Fixpoint subset (l : list nat) (m: list nat) : Prop := match l with
-  | nil => True
-  | cons x xs => elem x m /\ subset xs m
-  end.
+Require Import List Basics EqNat Logic.Decidable.
+Require Import Arith.Peano_dec.
+Require Import CpdtTactics.
 
 Lemma wrap : forall A B (f:A -> B), f = fun a:A => f a. auto. Qed.  
 
-Lemma subset_nil : forall ms, subset nil ms.
-intros. simpl. apply I. Qed.
+Fixpoint subset {A} (l : list A) (m: list A) : Prop := match l with
+  | nil => True
+  | cons x xs => In x m /\ subset xs m
+  end.
 
-Lemma or_false : forall t:Prop, (False \/ t) -> t.
-intros. intros. destruct H. inversion H. assumption. Qed.
+Lemma or_imp : forall a b c : Prop, (a \/ b -> c) <-> (a -> c) /\ (b -> c).
+intros. split; intros. split; intros.  apply or_introl with (B:=b) in H0. apply H in H0.
+assumption. apply or_intror with (A:=a) in H0. apply H in H0. assumption.
+destruct H. destruct H0. apply H in H0. assumption.  apply H1 in H0. assumption.
+Qed.
 
-Lemma subset_filter : forall l m f, subset m l -> subset (filter f m) l .
-intros. induction m. 
-  apply subset_nil. 
+Definition subset' {A} (l m : list A) : Prop := forall a, In a l -> In a m.
 
-  simpl in H. simpl. destruct (f a). unfold subset. split. destruct H.
-  assumption. destruct H. apply IHm in H0. assumption. destruct H. apply IHm in
-  H0. assumption. Qed.
+Definition forall_and {A} : forall (x y:A -> Prop), (forall a:A, x a /\ y a) <-> (forall
+a:A, x a) /\ (forall a:A, y a).
+intros. split;  intros. split; intros; specialize H with a; destruct H; assumption. 
+destruct H.  specialize H with a. specialize H0 with a. split; assumption. Qed.
+
+Definition forall_or {A} : forall (x y z:A -> Prop), (forall a:A, x a \/ y a -> z a) <-> (forall
+a:A, x a -> z a) /\ (forall a:A, y a -> z a).
+intros. split;  intros. split; intros. apply or_introl with (B:=y a) in H0.
+apply H in H0. assumption. apply or_intror with (A:=x a) in H0. apply H in H0.
+assumption. destruct H. destruct H0. apply H in H0. assumption. apply H1 in H0.
+assumption. Qed.
+
+Lemma subset'_cons {A} : forall (x : A) (l m : list A), 
+  subset' (x::l) m -> subset' l m.
+intros.  unfold subset' in H. unfold In at 1 in H. setoid_rewrite or_imp in H.
+apply forall_and in H. destruct H. assumption. Qed. 
+
+Lemma subset_eq : forall A (l m : list A), subset' l m <-> subset l m.
+intros. induction l. split. intros. unfold subset. auto. intros. unfold subset'.
+intros. inversion H0. split; intros. assert (In a (a::l)). unfold In. left.
+reflexivity. apply H in H0. unfold subset. split. assumption. 
+assert (subset' l m). apply subset'_cons in H. assumption. rewrite IHl in H1.
+assumption. unfold subset'. unfold subset in H. destruct H. rewrite <- IHl in
+H0. unfold In at 1. setoid_rewrite or_imp. rewrite forall_and. split. intros.
+rewrite <- H1. assumption. assumption. Qed.
+
+Lemma subset_nil : forall A ms, subset (@nil A) ms.
+intros. unfold subset. auto. Qed. 
+
+Lemma subset_nil2 : forall A ms, subset ms (@nil A) -> ms = nil.
+intros. rewrite <- subset_eq in H. unfold subset' in H. induction ms.
+reflexivity. simpl in H. specialize H with a. destruct H. left. reflexivity.
+Qed. 
+
+Fixpoint remove (x : nat) (l : list nat) := match l with
+  | nil => nil
+  | cons y ys => if eq_nat_dec x y then remove x ys else y::remove x ys
+  end.
+
+Lemma remove_in : forall (n : nat) ns, ~ In n (remove n ns).
+intros. induction ns. auto. unfold remove. destruct (eq_nat_dec n a).
+assumption. fold remove. unfold In. unfold not. rewrite not_or_iff. split.
+intros. symmetry in H. apply n0 in H. assumption. assumption. Qed.
+
+Lemma remove_app : forall (n : nat) ns ms, remove n (ns ++ ms) = remove n ns ++
+remove n ms.
+intros. induction ns. auto. simpl. rewrite IHns. destruct (eq_nat_dec n a).
+auto.  apply app_comm_cons. Qed. 
+
+Lemma remove_idem : forall (n : nat) ns, remove n (remove n ns) = remove n ns.
+intros. induction ns. simpl. auto. simpl. destruct (eq_nat_dec n a). assumption. 
+simpl. destruct (eq_nat_dec n a). apply n0 in e.  inversion e. rewrite IHns.
+reflexivity. Qed. 
+
+Lemma eq_nat_dec_refl : forall m, eq_nat_dec m m = left eq_refl.
+intros. induction m. auto. simpl. rewrite IHm. simpl. reflexivity. Qed. 
+
+Lemma remove_dup : forall (n m : nat) ns, remove n (remove m ns) = remove m
+(remove n ns).
+intros. induction ns. auto. simpl. destruct (eq_nat_dec m a). destruct
+(eq_nat_dec n a). rewrite e. rewrite e0. reflexivity. rewrite IHns. rewrite e.
+simpl. rewrite eq_nat_dec_refl. reflexivity. destruct (eq_nat_dec n a). rewrite
+e. simpl. rewrite eq_nat_dec_refl. rewrite <- e. rewrite IHns. reflexivity.
+simpl. destruct (eq_nat_dec n a). apply n1 in e. inversion e. destruct
+(eq_nat_dec m a). apply n0 in e. inversion e. rewrite IHns. reflexivity. Qed. 
+
+Lemma or_false : forall p : Prop, p \/ False <-> p. intros. split; intros.
+destruct H. assumption. inversion H. apply or_introl.  assumption. Qed.
+
+Lemma remove_not_in : forall (n v : nat) ns, n <> v -> (In n (remove v ns) <-> In n ns).
+intros. induction ns.  split; intros; inversion H0. split; intros; simpl. simpl
+in H0. destruct (eq_nat_dec v a). apply IHns in H0. right. assumption. simpl in
+H0. destruct H0. left; assumption. apply IHns in H0. right. assumption. destruct
+(eq_nat_dec v a). rewrite IHns. simpl in H0. destruct H0. rewrite H0 in e.
+symmetry in e. apply H in e. inversion e. assumption. simpl. simpl in H0.
+destruct H0. left. assumption. right. rewrite <- IHns in H0. assumption. Qed.
+
+Lemma subset_tail : forall (xs ys:list nat), subset xs (tl ys) -> subset xs ys.
+intros. induction xs. auto. simpl in H. simpl. destruct H. split. destruct ys.
+auto. simpl in H. apply in_cons. assumption. apply IHxs in H0. assumption. Qed. 
+
+Lemma noteq_comm {A} : forall (m n : A), m <> n -> n <> m.
+intros. auto. Qed. 
+
+Lemma beq_nat_comm : forall m n, beq_nat n m = beq_nat m n. 
+intros. destruct (eq_nat_dec m n).  rewrite e. reflexivity. assert (n <> m).
+apply noteq_comm in n0. assumption. apply
+beq_nat_false_iff in n0. apply beq_nat_false_iff in H. rewrite n0. rewrite H.
+reflexivity. Qed.
 
 Lemma let_inline : forall A (b c:A) f, f (let a := b in c) -> let a := b in (f c).
 auto. Qed.
 
-Lemma subset_singleton : forall x xs y, subset (x::xs) (y::nil) -> x = y.
-intros. inversion H. destruct H0. assumption. inversion H0. Qed.
+Lemma subset_singleton : forall (x y : nat) xs, subset (x::xs) (y::nil) -> x = y.
+intros. inversion H. destruct H0. symmetry. assumption. inversion H0. Qed.
 
-Lemma neq_bool_taut : forall m, neq_bool m m = true. intro. induction m. auto.
-auto. Qed.
+Lemma subset_cons {A} : forall (x : A) a l, subset a l -> subset a (x::l). intros.
+induction a. auto. inversion H. split. apply in_cons. assumption. 
+apply IHa in H1. assumption. Qed.  
 
-Lemma subset_cons : forall a x, subset a nil -> subset a (x::nil). intros.
-induction a. auto. inversion H. inversion H0. Qed. 
+Lemma cons_subset {A} : forall (x: A) xs ys, subset xs ys -> subset (x::xs) (x::ys).
+intros. unfold subset. simpl. split. left. reflexivity. apply subset_cons.
+assumption. Qed. 
 
-Lemma cons_subset : forall x xs ys, subset (x::xs) ys -> subset xs ys. intros.
-inversion H. assumption. Qed. 
+Lemma subset_remove : forall n ns, subset (remove n ns) ns.
+intros. induction ns. apply subset_nil. unfold remove. destruct (eq_nat_dec n
+a). fold remove. apply subset_cons. assumption. fold remove. apply cons_subset.
+assumption. Qed.
 
-Lemma subset_filter_cons : forall a v vs, subset a (v::vs) -> subset (filter
-(compose negb (neq_bool v)) a) vs. 
-intros. induction a. auto. inversion H. apply IHa in H1. inversion H0. rewrite
-H2.  unfold filter. unfold compose. rewrite neq_bool_taut. simpl. assumption. 
-unfold filter.  destruct (compose negb (neq_bool v) a). simpl. split.
-assumption. assumption. assumption. Qed.
+Lemma subset_in_cons : forall (n:nat) ns ms, ~In n ns -> subset ns (n::ms) -> subset ns ms. 
+intros.  rewrite <- subset_eq. rewrite <- subset_eq in H0. unfold subset' in
+H0. unfold In in H0 at 2. unfold subset'. intros. specialize H0 with a. 
+destruct (eq_nat_dec n a). rewrite <- e in H1. unfold not in H. apply H in H1.
+inversion H1. apply H0 in H1. destruct H1. apply n0 in H1. inversion H1.
+assumption. Qed. 
+
+Lemma symmetry : forall p q : Prop, p = q <-> q = p. intros. split; intros;
+symmetry in H; assumption. Qed. 
+
+Lemma subset_remove_cons : forall a v vs, subset a (v::vs) <-> subset (remove v a) vs. 
+intros. split; intros. rewrite <- subset_eq. rewrite <- subset_eq in H. unfold subset' in H.  
+unfold subset'. simpl in H. intros. specialize H with a0. destruct (eq_nat_dec
+a0 v). rewrite e in H. rewrite e in H0. apply remove_in in H0. inversion H0.
+assert (a0 <> v). assumption.  apply remove_not_in with (ns:=a) in n. rewrite n
+in H0. apply H in H0. destruct H0. symmetry in H0. apply H1 in H0. inversion H0.
+assumption.  rewrite <- subset_eq in H. unfold subset' in H. induction a. apply
+subset_nil.  simpl. split. simpl in H. destruct (eq_nat_dec v a). left.
+assumption. simpl in H. specialize H with a. assert (a = a).  reflexivity. apply
+or_introl with (B:=In a (remove v a0)) in H0. apply H in H0. right. assumption.
+simpl in H.  destruct (eq_nat_dec v a). apply IHa in H. assumption. simpl in H.
+rewrite forall_or in H. destruct H. apply IHa in H0. assumption. 
+Qed.
+
 
 Lemma truand : forall a:Prop, True /\ a -> a.
 intros. destruct H. auto. Qed. 
 
-Lemma app_subset : forall xs ys zs, subset (xs ++ ys) zs <-> (subset xs zs /\
- subset ys zs).
+Lemma app_subset_and {A} : forall xs ys zs: list A, subset (xs ++ ys) zs <-> (subset xs zs /\ subset ys zs).
 intros. 
 induction xs. simpl. 
 split. intros. auto. intros. destruct H. assumption. 
@@ -74,8 +169,41 @@ apply IHxs.
 split. unfold subset in H. destruct H. assumption. assumption. 
 Qed.
 
-Lemma elem_cons : forall n vs, elem n vs -> exists ms ns, vs = (ms ++ (n :: ns)).
-intros. induction vs. inversion H. unfold elem in H. inversion H. apply ex_intro
-with nil. apply ex_intro with vs. rewrite app_nil_l. rewrite H0. reflexivity.
-apply IHvs in H0. destruct H0. destruct H0. apply ex_intro with (a::x). apply
-ex_intro with x0. rewrite <- app_comm_cons. rewrite H0. reflexivity. Qed. 
+Lemma subset_id {A} : forall xs:list A, subset xs xs. 
+intros. induction xs. unfold subset. auto. unfold subset. split. unfold In.
+auto. apply subset_cons. auto. Qed. 
+
+Lemma subset_app_id {A} : forall xs ys zs:list A, subset ys zs -> subset (xs ++ ys) (xs ++ zs) .
+intros. induction xs. simpl. assumption. unfold subset. simpl. split. left.
+reflexivity. apply subset_cons. assumption. Qed.   
+
+Lemma subset_app {A} : forall xs ys zs:list A, subset xs ys -> subset xs (ys ++ zs).
+intros. rewrite <- subset_eq. rewrite <- subset_eq in H. unfold subset'. intros. rewrite
+in_app_iff.  left. apply H in H0.  assumption. Qed. 
+
+Lemma cons_app {A}: forall (x:A) xs, x :: xs = x::nil ++ xs.
+intros. rewrite app_nil_l. reflexivity. Qed.
+
+Lemma subset_comm1 {A} : forall xs ys zs:list A, subset (xs ++ ys) zs -> subset (ys ++ xs) zs.
+intros. apply app_subset_and. apply and_comm. apply app_subset_and. assumption.
+Qed. 
+
+Lemma subset_comm2 {A} : forall xs ys zs:list A, subset xs (ys ++ zs) -> subset xs (zs ++ ys). 
+intros. induction xs. auto. simpl. split. simpl in H. destruct H. apply
+in_app_or in H. apply or_comm in H. apply in_or_app in H. assumption. simpl in
+H. destruct H. apply IHxs in H0. assumption. Qed. 
+
+Lemma subset_trans {A}: forall xs ys zs:list A, subset xs ys -> subset ys zs -> subset xs zs. 
+intros. induction xs. unfold subset. auto. split. destruct H. rewrite <- subset_eq
+in H0. unfold subset' in H0. apply H0 in H. assumption. simpl in H. destruct H.
+apply IHxs in H1. assumption. Qed. 
+
+Definition set_equiv {A} (xs ys : list A) : Prop := subset xs ys /\ subset ys xs. 
+
+Lemma subset_swap {A} : forall (n v : A) vs, set_equiv (n::v::vs) (v::n::vs).
+intros. unfold set_equiv. simpl. split; split. right. left. reflexivity. split.
+left. reflexivity. repeat (apply subset_cons). apply subset_id. right. left.
+reflexivity. split. left. reflexivity. repeat (apply subset_cons). apply
+subset_id. Qed.
+
+
